wip

Semantic/Stlc/Interpreter.lean
@@ -80,3 +80,53 @@ def eval : Store n -> Exp n -> Nat -> EvalResult n
     | _ => .stuck
   | .stuck => .stuck
   | .timeout => .timeout
+
+structure Config (n : Nat) where
+  s : Store n
+  e : Exp n
+
+def EvalResult.rename : EvalResult n1 -> (f : Rename n1 n2) -> EvalResult n2
+| .ok v, f => .ok (v.rename f)
+| .stuck, _ => .stuck
+| .timeout, _ => .timeout
+
+inductive Eval : Store n -> Exp n -> Exp n -> Prop where
+| ev_var :
+  Eval s (.var x) (s.lookup x)
+| ev_abs :
+  Eval s (.abs T e) (.abs T e)
+| ev_app :
+  Eval s e1 (.abs T ebody) ->
+  Eval s e2 v2 ->
+  Eval (Store.val s v2) ebody eres ->
+  Eval s (.app e1 e2) (eres.subst (Subst.openVar v2))
+| ev_btrue :
+  Eval s .btrue .btrue
+| ev_bfalse :
+  Eval s .bfalse .bfalse
+| ev_nzero :
+  Eval s .nzero .nzero
+| ev_nsucc :
+  Eval s e v ->
+  v.is_num_val ->
+  Eval s (.nsucc e) (.nsucc v)
+| ev_pred_nzero :
+  Eval s (.pred .nzero) .nzero
+| ev_pred_nsucc :
+  Eval s e (.nsucc v) ->
+  v.is_num_val ->
+  Eval s (.pred (.nsucc v)) v
+| ev_iszero_nzero :
+  Eval s (.iszero .nzero) .btrue
+| ev_iszero_nsucc :
+  Eval s e (.nsucc v) ->
+  v.is_num_val ->
+  Eval s (.iszero (.nsucc v)) .bfalse
+| ev_cond_true :
+  Eval s e1 .btrue ->
+  Eval s e2 v2 ->
+  Eval s (.cond e1 e2 e3) v2
+| ev_cond_false :
+  Eval s e1 .bfalse ->
+  Eval s e3 v3 ->
+  Eval s (.cond e1 e2 e3) v3
