Semantic/Stlc/RebindTheory.lean
@@ -1,0 +1,41 @@
+import Semantic.Stlc.TypeSystem
+import Semantic.Stlc.Interpreter
+import Mathlib.Tactic
+
+def hello : Nat := 42
+
+structure Rebind (s1 : Store n1) (f : Rename n1 n2) (s2 : Store n2) where
+  var : ∀ (x : Var n1),
+    s2.lookup (f.var x) = (s1.lookup x).rename f
+
+theorem eval_rebind {f : Rename n1 n2}
+  (ρ : Rebind s1 f s2)
+  (e : Exp n1) :
+  eval s2 (e.rename f) fuel = (eval s1 e fuel).rename f := by
+  induction e generalizing fuel s2
+  case var x0 =>
+    cases fuel
+    case zero => rfl
+    case succ fuel =>
+      simp [Exp.rename, eval]
+      have := ρ.var x0
+      grind [EvalResult.rename]
+  case abs ih =>
+    cases fuel
+    case zero => rfl
+    case succ fuel =>
+      simp [Exp.rename, eval]
+      grind [EvalResult.rename, Exp.rename]
+  case app ih1 ih2 =>
+    cases fuel
+    case zero => rfl
+    case succ fuel =>
+      conv => lhs; simp [Exp.rename]
+      sorry
+  case btrue => sorry
+  case bfalse => sorry
+  case nzero => sorry
+  case nsucc => sorry
+  case pred => sorry
+  case iszero => sorry
+  case cond => sorry
